theories/lang/cpp/logic/func.v
@@ -1,5 +1,5 @@
 (*
- * Copyright (C) BedRock Systems Inc. 2019 Gregory Malecha
+ * Copyright (C) BedRock Systems Inc. 2019-2020 Gregory Malecha
  *
  * SPDX-License-Identifier:AGPL-3.0-or-later
  *)
@@ -13,97 +13,17 @@ Require Import stdpp.telescopes.
 From iris.proofmode Require Import tactics.
 From bedrock Require Import ChargeUtil ChargeCompat.
 
-From bedrock.lang.cpp Require Import ast semantics.
+From bedrock.lang.cpp Require Import ast semantics spec.
 From bedrock.lang.cpp Require Import
      pred path_pred heap_pred
      wp intensional.
 
 Local Open Scope string_scope.
 
-
 Local Set Universe Polymorphism.
 
-Module Type Func.
-
-  Section with_prop.
-    Context {PROP : bi}.
-
-    Record WithEx@{X Z Y} : Type :=
-      { we_ex   : tele@{X}
-      ; we_post : tele_fun@{X Z Y} we_ex (val * PROP) }.
-
-    Definition WithEx_map (f : val -> PROP -> val * PROP) (we : WithEx) : WithEx :=
-      {| we_ex := we.(we_ex)
-       ; we_post := tele_map (fun '(r,Q) => f r Q) we.(we_post) |}.
-
-    Record WithPrePost@{X Z Y} : Type :=
-      { wpp_with : tele@{X}
-      ; wpp_pre  : tele_fun@{X Z Y} wpp_with (list val * PROP)
-      ; wpp_post : tele_fun@{X Z Y} wpp_with WithEx@{X Z Z} }.
-
-    Fixpoint tbi_exist@{X Z Y} {t : tele@{X}} : forall (P : tele_fun@{X Z Y} t PROP), PROP :=
-      match t as t0 return ((t0 -t> PROP) → PROP) with
-      | [tele] => fun x : PROP => x
-      | @TeleS X binder =>
-        fun P : (∀ x : X, binder x -t> PROP) => Exists x : X, tbi_exist (P x)
-      end.
-
-    Fixpoint tbi_forall@{X Z Y} {t : tele@{X}} : forall (P : tele_fun@{X Z Y} t PROP), PROP :=
-      match t as t0 return ((t0 -t> PROP) → PROP) with
-      | [tele] => fun x : PROP => x
-      | @TeleS X binder =>
-        fun P : (∀ x : X, binder x -t> PROP) => Forall x : X, tbi_forall (P x)
-      end.
-
-    Definition WppD@{X Z Y} (wpp : WithPrePost@{X Z Y}) (params : list val) (Q : val -> PROP) : PROP :=
-      tbi_exist@{X Z Y} (tele_bind (TT:=wpp.(wpp_with)) (fun args =>
-         let P := tele_app wpp.(wpp_pre) args in
-         let Q' := tele_app wpp.(wpp_post) args in
-         [| params = fst P |] ** snd P **
-         tbi_forall@{X Z Y} (tele_map (fun '(result,Q') => Q' -* Q result) Q'.(we_post)))).
-
-  End with_prop.
-  Arguments WithPrePost : clear implicits.
-  Arguments Build_WithPrePost _ _ _ : clear implicits.
-  Arguments WithEx : clear implicits.
-  Arguments Build_WithEx _ _ _ : clear implicits.
-
-  Arguments we_ex {PROP} _.
-  Arguments we_post {PROP} _.
-  Arguments wpp_with {_} _.
-  Arguments wpp_pre {_} _.
-  Arguments wpp_post {_} _.
-
-  Global Arguments WppD !_ / .
-
-  Section with_cpp.
+Section with_cpp.
   Context `{Σ : cpp_logic thread_info} {resolve:genv}.
-
-    Record function_spec : Type :=
-      { fs_return : type
-      ; fs_arguments : list type
-      ; fs_spec : thread_info -> list val -> (val -> mpred) -> mpred
-      }.
-  Arguments function_spec : clear implicits.
-  Arguments Build_function_spec : clear implicits.
-
-  (* function specifications written in weakest pre-condition style.
-   *)
-
-  Definition type_of_spec `(fs : function_spec) : type :=
-    normalize_type (Tfunction fs.(fs_return) fs.(fs_arguments)).
-
-  (* this is the core definition that everything will be based on.
-   * it is really an assertion about assembly
-   *)
-  Definition cptr_def (fs : function_spec) : Rep :=
-    as_Rep (fun p =>
-         Forall vs,
-         [| List.length vs = List.length fs.(fs_arguments) |] -*
-         Forall Q (ti : thread_info), fs.(fs_spec) ti vs Q -* fspec ti (Vptr p) vs Q).
-  Definition cptr_aux : seal (@cptr_def). by eexists. Qed.
-  Definition cptr := cptr_aux.(unseal).
-  Definition cptr_eq : @cptr = _ := cptr_aux.(seal_eq).
 
   (* Hoare triple for a function.
    * note(gmm): these should include linkage specifications.
@@ -179,12 +99,8 @@ Module Type Func.
                    tele_map (map_pre (Vptr this)) (PQ this).(wpp_pre)
                ; wpp_post this := (PQ this).(wpp_post)
                |}.
-      (* ^ todo(gmm): this looks wrong. something isn't going
-       * to fit together with respect to calling conventions and
-       * specifications.
-       *)
 
-  Local Definition local_addr_v (r : region) (x : ident) (v : val) : mpred :=
+  Let local_addr_v (r : region) (x : ident) (v : val) : mpred :=
     Exists p, [| v = Vptr p |] ** local_addr r x p.
 
   Fixpoint bind_type ρ (t : type) (x : ident) (v : val) : mpred :=
@@ -205,19 +121,19 @@ Module Type Func.
     | _              => Exists a, tlocal_at ρ x a (anyR (erase_qualifiers t) 1)
     end.
 
-  Fixpoint ForallEaches (ts : list type) : (list (type * val) -> mpred) -> mpred :=
+  Fixpoint Forall_with_type (ts : list type) : (list (type * val) -> mpred) -> mpred :=
     match ts with
     | nil => fun k => k nil
-    | t :: ts => fun k => Forall v : val, ForallEaches ts (fun args => k ((t,v) :: args))
+    | t :: ts => fun k => Forall v : val, Forall_with_type ts (fun args => k ((t,v) :: args))
     end.
 
-    (* the proof obligation for a function
-     *)
-
-  Definition wp_func (f : Func) (ti : thread_info) (args : list val) (Q : val -> epred) : mpred :=
+  (* the meaning of a function
+   *)
+  Definition wp_func (f : Func) (ti : thread_info) (args : list val)
+             (Q : val -> epred) : mpred :=
     match f.(f_body) with
-      | None => lfalse
-      | Some body =>
+    | None => lfalse
+    | Some body =>
         let ret := f.(f_return) in
         Forall ρ : region,
         (* this is what is created from the parameters *)
@@ -240,237 +156,146 @@ Module Type Func.
           wp (resolve:=resolve) ti ρ body (Kfree frees (val_return (fun x => |> Q x)))
       end.
 
-  Definition wp_method (meth : Method) ti (args : list val) (Q : val -> epred) : mpred :=
-      match meth.(m_body) with
-      | None => lfalse
-      | Some body =>
-          Forall ρ : region,
-          match args with
-          | this_val :: rest_vals =>
-            Forall thisp, [| this_val = Vptr thisp |] -*
-            (* this is what is created from the parameters *)
-            let binds :=
-                this_addr ρ thisp **
-                sepSPs (zip_with (fun '(x, t) 'v => bind_type ρ t x v) meth.(m_params) rest_vals)
-            in
-            (* this is what is freed on return *)
-            let frees :=
-                this_addr ρ thisp **
-                sepSPs (zip_with (fun '(x, t) 'v => free_type ρ t x v) (rev meth.(m_params))
-                       (rev rest_vals))
-            in
-            let ret_ty := meth.(m_return) in
-            ([| (length args = 1 + length meth.(m_params))%nat |] ** ltrue) //\\
-            if is_void ret_ty
-            then
-              binds -* (wp (resolve:=resolve) ti ρ body (Kfree frees (void_return (|>Q Vvoid))))
-            else if is_aggregate ret_ty then
-              Forall ra,
-              (binds ** result_addr ρ ra ** _at (_eq ra) (uninitR (erase_qualifiers ret_ty) 1)) -* (wp (resolve:=resolve) ti ρ body (Kfree (frees ** result_addr ρ ra) (val_return (fun x => |>Q x))))
-            else
-              binds -* (wp (resolve:=resolve) ti ρ body (Kfree frees (val_return (fun x => |>Q x))))
-          | _ => lfalse
-          end
-      end.
-    (* ^ todo(gmm): move the [frees] to the left hand side of the [-*], this
-     * will make the right-hand-side more canonical
-     *)
-
-    (* todo(gmm): i should be able to define this using [wp_func] *)
-    Definition func_ok (f : Func)
-               (ti : thread_info) (spec : function_spec)
+  Definition func_ok (f : Func) (ti : thread_info) (spec : function_spec)
     : mpred :=
-      match f.(f_body) with
-      | None => lfalse
-      | Some body =>
-        let params := f.(f_params) in
-        let ret := f.(f_return) in
-      [| type_of_spec spec = normalize_type (Tfunction ret (List.map snd params)) |] **
+      [| type_of_spec spec =
+         normalize_type (Tfunction f.(f_return) (List.map snd f.(f_params))) |] **
       (* forall each argument, apply to [fs_spec ti] *)
-      ForallEaches (spec.(fs_arguments)) (fun args =>
-        Forall ρ : region,
-        let vals := List.map snd args in
-        let PQ := spec.(fs_spec) ti vals in
+      □ Forall Q : val -> mpred, Forall vals,
+        spec.(fs_spec) ti vals Q -* wp_func f ti vals Q.
 
+  Definition wp_method (meth : Method) ti (args : list val)
+             (Q : val -> epred) : mpred :=
+    match meth.(m_body) with
+    | None => lfalse
+    | Some body =>
+      Forall ρ : region,
+      match args with
+      | this_val :: rest_vals =>
+        Forall thisp, [| this_val = Vptr thisp |] -*
         (* this is what is created from the parameters *)
         let binds :=
-            sepSPs (zip_with (fun '(x, t) 'v => bind_type ρ t x v) params vals) in
+            this_addr ρ thisp **
+            sepSPs (zip_with (fun '(x, t) 'v => bind_type ρ t x v) meth.(m_params) rest_vals)
+        in
         (* this is what is freed on return *)
         let frees :=
-            sepSPs (zip_with (fun '(x, t) 'v => free_type ρ t x v)
-                   (rev params) (rev vals)) in
-        if is_void ret
+            this_addr ρ thisp **
+            sepSPs (zip_with (fun '(x, t) 'v => free_type ρ t x v) (rev meth.(m_params))
+                             (rev rest_vals))
+        in
+        let ret_ty := meth.(m_return) in
+        ([| (length args = 1 + length meth.(m_params))%nat |] ** ltrue) //\\
+        if is_void ret_ty
         then
-          Forall Q : mpred,
-          (binds ** PQ (fun x => Q)) -*
-          wp (resolve:=resolve) ti ρ body (Kfree frees (void_return (|>Q)))
-        else if is_aggregate ret then
-          Forall Q : val -> mpred,
+          binds -* (wp (resolve:=resolve) ti ρ body (Kfree frees (void_return (|>Q Vvoid))))
+        else if is_aggregate ret_ty then
           Forall ra,
-          (binds ** result_addr ρ ra ** _at (_eq ra) (uninitR (erase_qualifiers ret) 1) ** PQ Q) -*
-          wp (resolve:=resolve) ti ρ body (Kfree (frees ** result_addr ρ ra) (val_return (fun x => |> Q x)))
+          (binds ** result_addr ρ ra ** _at (_eq ra) (uninitR (erase_qualifiers ret_ty) 1)) -* (wp (resolve:=resolve) ti ρ body (Kfree (frees ** result_addr ρ ra) (val_return (fun x => |>Q x))))
         else
-          Forall Q : val -> mpred,
-          (binds ** PQ Q) -*
-          wp (resolve:=resolve) ti ρ body (Kfree frees (val_return (fun x => |> Q x))))
-      end.
-    (* ^ todo(gmm): the new semantics of function gets an address for a return value
-     * so the semantics for `return` should be that *)
+          binds -* (wp (resolve:=resolve) ti ρ body (Kfree frees (val_return (fun x => |>Q x))))
+      | _ => lfalse
+      end
+    end.
 
-
-
-    Definition method_ok (meth : Method) (ti : thread_info) (spec : function_spec)
-      : mpred :=
-      match meth.(m_body) with
-      | None => lfalse
-      | Some body =>
-        let this_type :=
-            Qconst (Tpointer (Tqualified meth.(m_this_qual) (Tnamed meth.(m_class))))
-        in
-        [| type_of_spec spec =
-           normalize_type (Tfunction meth.(m_return) (this_type :: List.map snd meth.(m_params))) |] **
-        ForallEaches spec.(fs_arguments) (fun args =>
-          Forall ρ : region,
-          let vals := List.map snd args in
-          let PQ := spec.(fs_spec) ti vals in
-          match vals with
-          | this_val :: rest_vals =>
-            Forall thisp, [| this_val = Vptr thisp |] -*
-            (* this is what is created from the parameters *)
-            let binds :=
-                this_addr ρ thisp **
-                sepSPs (zip_with (fun '(x, t) 'v => bind_type ρ t x v) meth.(m_params) rest_vals)
-            in
-            (* this is what is freed on return *)
-            let frees :=
-                this_addr ρ thisp **
-                sepSPs (zip_with (fun '(x, t) 'v => free_type ρ t x v) (rev meth.(m_params))
-                       (rev rest_vals))
-            in
-            let ret_ty := meth.(m_return) in
-            if is_void ret_ty
-            then
-              Forall Q : mpred,
-              (binds ** PQ (fun x => Q)) -* (wp (resolve:=resolve) ti ρ body (Kfree frees (void_return (|>Q))))
-            else if is_aggregate ret_ty then
-              Forall Q : val -> mpred,
-              Forall ra,
-              (binds ** result_addr ρ ra ** _at (_eq ra) (uninitR (erase_qualifiers ret_ty) 1) ** PQ Q) -* (wp (resolve:=resolve) ti ρ body (Kfree (frees ** result_addr ρ ra) (val_return (fun x => |>Q x))))
-            else
-              Forall Q : val -> mpred,
-              (binds ** PQ Q) -* (wp (resolve:=resolve) ti ρ body (Kfree frees (val_return (fun x => |>Q x))))
-          | _ => lfalse
-          end)
-      end.
-    (* ^ todo(gmm): move the [frees] to the left hand side of the [-*], this
-     * will make the right-hand-side more canonical
-     *)
-
-    Fixpoint wpis (ti : thread_info) (ρ : region) (cls : globname) (this : val)
-             (inits : list Initializer)
-             (Q : mpred -> mpred) : mpred :=
-      match inits with
-      | nil => Q empSP
-      | i :: is' => wpi (resolve:=resolve) ti ρ cls this i (fun f => f ** wpis ti ρ cls this is' Q)
-      end.
-
-
-    Definition wp_ctor (cls : globname) (ti : thread_info) (ρ : region)
-               (this_val : val)
-               (inits : list Initializer) (body : Stmt)
-               (Q : Kpreds)
+  Definition method_ok (m : Method) (ti : thread_info) (spec : function_spec)
     : mpred :=
-      wpis ti ρ cls this_val inits
-           (fun free => free ** wp (resolve:=resolve) ti ρ body Q).
+    [| type_of_spec spec =
+       normalize_type (Tfunction m.(m_return) (Tpointer (Tqualified m.(m_this_qual) (Tnamed m.(m_class))) :: List.map snd m.(m_params))) |] **
+    (* forall each argument, apply to [fs_spec ti] *)
+    □ Forall Q : val -> mpred, Forall vals,
+      spec.(fs_spec) ti vals Q -* wp_method m ti vals Q.
 
 
-    Definition ctor_ok (ctor : Ctor) (ti : thread_info) (spec : function_spec)
-    : mpred :=
-      match ctor.(c_body) with
-      | None => lfalse
-      | Some Defaulted => lfalse
+  Fixpoint wpis (ti : thread_info) (ρ : region) (cls : globname) (this : val)
+           (inits : list Initializer)
+           (Q : mpred -> mpred) : mpred :=
+    match inits with
+    | nil => Q empSP
+    | i :: is' => wpi (resolve:=resolve) ti ρ cls this i (fun f => f ** wpis ti ρ cls this is' Q)
+    end.
+
+  Definition wp_ctor (ctor : Ctor) (ti : thread_info) (args : list val)
+             (Q : val -> epred) : mpred :=
+    match ctor.(c_body) with
+    | None => lfalse
+    | Some Defaulted => lfalse
       (* ^ defaulted constructors are not supported yet *)
-      | Some (UserDefined (init, body)) =>
-        let this_type :=
-            Qconst (Tpointer (Qmut (Tnamed ctor.(c_class))))
+    | Some (UserDefined (inits, body)) =>
+      let this_type :=
+          Qconst (Tpointer (Qmut (Tnamed ctor.(c_class))))
+      in
+      Forall ρ,
+      match args with
+      | this_val :: rest_vals =>
+        Forall thisp, [| this_val = Vptr thisp |] -*
+        (* this is what is created from the parameters *)
+        let binds :=
+            this_addr ρ thisp **
+            sepSPs (zip_with (fun '(x, t) 'v => bind_type ρ t x v) ctor.(c_params) rest_vals)
         in
-        [| type_of_spec spec =
-           normalize_type (Tfunction Tvoid (this_type :: List.map snd ctor.(c_params))) |] **
-        ForallEaches spec.(fs_arguments) (fun args =>
-          Forall ρ,
-          let vals := List.map snd args in
-          let PQ := spec.(fs_spec) ti vals in
-          match vals with
-          | this_val :: rest_vals =>
-            Forall thisp, [| this_val = Vptr thisp |] -*
-            (* this is what is created from the parameters *)
-            let binds :=
-                this_addr ρ thisp **
-                sepSPs (zip_with (fun '(x, t) 'v => bind_type ρ t x v) ctor.(c_params) rest_vals)
-            in
-            (* this is what is freed on return *)
-            let frees :=
-                this_addr ρ thisp **
-                sepSPs (zip_with (fun '(x, t) 'v => free_type ρ t x v) (rev ctor.(c_params)) (rev rest_vals))
-            in
-            Forall Q : mpred,
-            (binds ** PQ (fun x => Q)) -*
-            (wp_ctor ctor.(c_class) ti ρ (Vptr thisp) init body
-                     (Kfree frees (void_return (|>Q))))
-          | _ => lfalse
-          end)
-      end.
+        (* this is what is freed on return *)
+        let frees :=
+            this_addr ρ thisp **
+            sepSPs (zip_with (fun '(x, t) 'v => free_type ρ t x v) (rev ctor.(c_params)) (rev rest_vals))
+        in
+        binds -*
+        wpis ti ρ ctor.(c_class) this_val inits
+           (fun free => free **
+                      wp (resolve:=resolve) ti ρ body (Kfree frees (void_return (|> Q Vvoid))))
+       | _ => lfalse
+      end
+    end.
 
-    Fixpoint wpds (ti : thread_info) (ρ : region)
-             (cls : globname) (this : val)
-             (dests : list (FieldOrBase * globname))
-             (Q : mpred) : mpred :=
-      match dests with
-      | nil => Q
-      | d :: ds => @wpd _ Σ resolve ti ρ cls this d (wpds ti ρ cls this ds Q)
-      end.
-
-
-    Definition wp_dtor (ti : thread_info) (ρ : region) (cls : globname)
-               (this_val : val)
-               (body : Stmt) (dtors : list (FieldOrBase * globname))
-               (frees : mpred) (Q : mpred)
+  Definition ctor_ok (ctor : Ctor) (ti : thread_info) (spec : function_spec)
     : mpred :=
-      @wp _ Σ resolve ti ρ body
-         (Kfree frees (void_return (wpds ti ρ cls this_val dtors Q))).
+    [| type_of_spec spec =
+       normalize_type (Tfunction Tvoid (Tpointer (Tnamed ctor.(c_class)) :: List.map snd ctor.(c_params))) |] **
+    (* forall each argument, apply to [fs_spec ti] *)
+    □ Forall Q : val -> mpred, Forall vals,
+      spec.(fs_spec) ti vals Q -* wp_ctor ctor ti vals Q.
 
-    Definition dtor_ok (dtor : Dtor) (ti : thread_info) (spec : function_spec)
-    : mpred :=
-      match dtor.(d_body) with
-      | None => lfalse
-      | Some Defaulted => lfalse
+  Fixpoint wpds (ti : thread_info) (ρ : region)
+           (cls : globname) (this : val)
+           (dests : list (FieldOrBase * globname))
+           (Q : mpred) : mpred :=
+    match dests with
+    | nil => Q
+    | d :: ds => @wpd _ Σ resolve ti ρ cls this d (wpds ti ρ cls this ds Q)
+    end.
+
+  Definition wp_dtor (dtor : Dtor) (ti : thread_info) (args : list val)
+             (Q : val -> epred) : mpred :=
+    match dtor.(d_body) with
+    | None => lfalse
+    | Some Defaulted => lfalse
       (* ^ defaulted constructors are not supported yet *)
-      | Some (UserDefined (body, deinit)) =>
-        let this_type :=
-            Qconst (Tpointer (Qmut (Tnamed dtor.(d_class))))
-        in
-        [| type_of_spec spec = normalize_type (Tfunction Tvoid (this_type :: nil)) |] **
-        ForallEaches spec.(fs_arguments) (fun args =>
-          Forall ρ,
-          let vals := List.map snd args in
-          let PQ := spec.(fs_spec) ti vals in
-          match vals with
-          | this_val :: rest_vals =>
-            Forall thisp, [| this_val = Vptr thisp |] -*
-            (* this is what is created from the parameters *)
-            let binds := this_addr ρ thisp in
-            (* this is what is freed on return *)
-            let frees := this_addr ρ thisp in
-            Forall Q : mpred,
-              (binds ** PQ (fun x => Q)) -*
-              (wp_dtor ti ρ dtor.(d_class) (Vptr thisp) body deinit frees (|>Q))
-          | _ => lfalse
-          end)
-      end.
-  End with_cpp.
+    | Some (UserDefined (body, deinit)) =>
+      let this_type :=
+          Qconst (Tpointer (Qmut (Tnamed dtor.(d_class))))
+      in
+      Forall ρ,
+      match args with
+      | this_val :: rest_vals =>
+        Forall thisp, [| this_val = Vptr thisp |] -*
+        (* this is what is created from the parameters *)
+        let binds := this_addr ρ thisp in
+        (* this is what is freed on return *)
+        let frees := this_addr ρ thisp in
+          binds -*
+          wp (resolve:=resolve) ti ρ body
+          (Kfree frees (void_return (wpds ti ρ dtor.(d_class) this_val deinit (|> Q Vvoid))))
+      | _ => lfalse
+      end
+    end.
 
-End Func.
 
-Declare Module F : Func.
+  Definition dtor_ok (dtor : Dtor) (ti : thread_info) (spec : function_spec)
+    : mpred :=
+    [| type_of_spec spec =
+       normalize_type (Tfunction Tvoid (Tpointer (Tnamed dtor.(d_class)) :: nil)) |] **
+    (* forall each argument, apply to [fs_spec ti] *)
+    □ Forall Q : val -> mpred, Forall vals,
+      spec.(fs_spec) ti vals Q -* wp_dtor dtor ti vals Q.
 
-Export F.
+End with_cpp.
