theories/lang/cpp/compile.v
@@ -1,0 +1,47 @@
+(*
+ * Copyright (C) BedRock Systems Inc. 2020
+ *
+ * SPDX-License-Identifier:AGPL-3.0-or-later
+ *)
+
+(** this file describes the assumptions made about the compiler.
+
+    in particular, it describes the connection between the semantics
+    of C++ declarations (e.g. functions, methods, constructors, destructors),
+    and the machine-level specification of the bytes in memory ([fspec]).
+
+ *)
+
+Require Import bedrock.lang.cpp.ast.
+Require Import bedrock.lang.cpp.logic.
+Require Import bedrock.lang.cpp.semantics.
+
+Section with_Σ.
+  Context `{Σ : cpp_logic thread_info}.
+  Context {ti : thread_info} {σ : genv}.
+
+  (** compilation of a function [f] is correct if the weakest pre-condition
+      of the function ([wp_func]) implies the weakest pre-condition of the
+      compiled code ([fspec]).
+   *)
+  Axiom code_at_ok : forall (f : Func) p,
+      code_at (σ:=σ) f p
+      |-- Forall ti ls Q, wp_func (resolve:=σ) f ti ls Q -*
+                          fspec ti (Vptr p) ls Q.
+
+  Axiom method_at_ok : forall (m : Method) p,
+      method_at (σ:=σ) m p
+      |-- Forall ti ls Q, wp_method (resolve:=σ) m ti ls Q -*
+                          fspec ti (Vptr p) ls Q.
+
+  Axiom ctor_at_ok : forall (c : Ctor) p,
+      ctor_at (σ:=σ) c p
+      |-- Forall ti ls Q, wp_ctor (resolve:=σ) c ti ls Q -*
+                          fspec ti (Vptr p) ls Q.
+
+  Axiom dtor_at_ok : forall (d : Dtor) p,
+      dtor_at (σ:=σ) d p
+      |-- Forall ti ls Q, wp_dtor (resolve:=σ) d ti ls Q -*
+                          fspec ti (Vptr p) ls Q.
+
+End with_Σ.
