theories/lang/cpp/logic.v
@@ -9,6 +9,7 @@ From bedrock.lang.cpp.logic Require Export
      pred
      path_pred
      heap_pred
+     spec
      wp
      intensional
      destroy
