theories/lang/cpp/logic/spec.v
@@ -1,0 +1,72 @@
+(*
+ * Copyright (C) BedRock Systems Inc. 2019 Gregory Malecha
+ *
+ * SPDX-License-Identifier:AGPL-3.0-or-later
+ *)
+Require Import Coq.Lists.List.
+
+Require Import stdpp.telescopes.
+
+From iris.proofmode Require Import tactics.
+
+From bedrock.lang.cpp Require Import ast semantics.
+From bedrock.lang.cpp Require Import pred.
+
+Local Open Scope string_scope.
+
+Local Set Universe Polymorphism.
+
+Section with_prop.
+  Context {PROP : bi}.
+
+  Record WithEx@{X Z Y} : Type :=
+    { we_ex   : tele@{X}
+    ; we_post : tele_fun@{X Z Y} we_ex (val * PROP) }.
+
+  Definition WithEx_map (f : val -> PROP -> val * PROP) (we : WithEx)
+    : WithEx :=
+    {| we_ex := we.(we_ex)
+     ; we_post := tele_map (fun '(r,Q) => f r Q) we.(we_post) |}.
+
+  Record WithPrePost@{X Z Y} : Type :=
+    { wpp_with : tele@{X}
+    ; wpp_pre  : tele_fun@{X Z Y} wpp_with (list val * PROP)
+    ; wpp_post : tele_fun@{X Z Y} wpp_with WithEx@{X Z Z} }.
+
+  Fixpoint tbi_exist@{X Z Y} {t : tele@{X}}
+    : forall (P : tele_fun@{X Z Y} t PROP), PROP :=
+    match t as t0 return ((t0 -t> PROP) → PROP) with
+    | [tele] => fun x : PROP => x
+    | @TeleS X binder =>
+      fun P : (∀ x : X, binder x -t> PROP) => Exists x : X, tbi_exist (P x)
+    end.
+
+  Fixpoint tbi_forall@{X Z Y} {t : tele@{X}}
+    : forall (P : tele_fun@{X Z Y} t PROP), PROP :=
+    match t as t0 return ((t0 -t> PROP) → PROP) with
+    | [tele] => fun x : PROP => x
+    | @TeleS X binder =>
+      fun P : (∀ x : X, binder x -t> PROP) => Forall x : X, tbi_forall (P x)
+    end.
+
+  Definition WppD@{X Z Y} (wpp : WithPrePost@{X Z Y}) (params : list val)
+             (Q : val -> PROP) : PROP :=
+    tbi_exist@{X Z Y} (tele_bind (TT:=wpp.(wpp_with)) (fun args =>
+      let P := tele_app wpp.(wpp_pre) args in
+      let Q' := tele_app wpp.(wpp_post) args in
+      [| params = fst P |] ** snd P **
+      tbi_forall@{X Z Y} (tele_map (fun '(result,Q') => Q' -* Q result) Q'.(we_post)))).
+
+End with_prop.
+Arguments WithPrePost : clear implicits.
+Arguments Build_WithPrePost _ _ _ : clear implicits.
+Arguments WithEx : clear implicits.
+Arguments Build_WithEx _ _ _ : clear implicits.
+
+Arguments we_ex {PROP} _.
+Arguments we_post {PROP} _.
+Arguments wpp_with {_} _.
+Arguments wpp_pre {_} _.
+Arguments wpp_post {_} _.
+
+Global Arguments WppD !_ / .
